a failed attempt on the na_inv+inv approach..

theories/RAs.v
@@ -1,23 +1,18 @@
 From iris.base_logic.lib Require Import gen_heap ghost_map invariants na_invariants.
-From iris.algebra Require Import auth agree dfrac csum excl gmap gmap_view gset frac_agree.
+From iris.algebra Require Import auth agree dfrac csum excl gmap gmap_view gset frac_agree frac_auth.
 From iris.proofmode Require Import tactics.
 From HypVeri Require Export lang machine.
 
   Class gen_VMPreG (A V W R P F: Type) (Σ:gFunctors)
         `{Countable A, Countable V, Countable W, Countable R, Countable P} := {
-                      (* gen_num_preG_inG :> inG Σ (agreeR natO); *)
-                      gen_token_preG_inG :> inG Σ (frac_agreeR (leibnizO V));
+                      gen_token_preG_inG :> inG Σ (frac_authR (agreeR (leibnizO V)));
                       gen_mem_preG_inG :> gen_heapGpreS A W Σ;
                       gen_reg_preG_inG :> gen_heapGpreS (R * V) W Σ;
                       gen_tx_preG_inG :> inG Σ (authR (gmapUR V (agreeR (leibnizO P))));
                       gen_rx_preG_inG :> inG Σ (prodR (authR (gmapUR V (agreeR (leibnizO P))))
                                                       (optionR (gmap_viewR V (optionO (prodO (leibnizO W) (leibnizO V))))));
-                      (* gen_owned_preG_inG :> inG Σ (authR (gset_disjUR (leibnizO P))); *)
-                      (* gen_access_preG_inG :> inG Σ (authR (gmapUR P (prodR dfracR (csumR (agreeR unitO) (exclR unitO))))); *)
                       gen_owned_preG_inG :> inG Σ (authR (gmapUR V
                                     (prodR dfracR (agreeR (gset_disjUR (leibnizO P))))));
-                      (* gen_access_preG_inG :> inG Σ (authR (gmapUR V *)
-                                    (* (prodR dfracR (gmapUR P (csumR (agreeR unitO) (exclR unitO)))))); *)
                       gen_access_preG_inG :> inG Σ (authR (gmapUR V
                                                     (prodR dfracR (agreeR (gset_disjUR (leibnizO P))))));
                       gen_trans_preG_inG :> gen_heapGpreS W (V * W* W*(gmap V (gset P))*F) Σ;
@@ -32,7 +27,6 @@ From HypVeri Require Export lang machine.
                       gen_na_invG :> na_invG Σ;
                       gen_nainv_name : na_inv_pool_name;
                       gen_token_name : gname;
-                      (* gen_num_name : gname; *)
                       gen_mem_name : gname;
                       gen_reg_name : gname;
                       gen_tx_name : gname;
@@ -44,7 +38,6 @@ From HypVeri Require Export lang machine.
                       gen_retri_name : gname
                     }.
 Global Arguments gen_nainv_name {Σ} _.
-(* Global Arguments gen_num_name {Σ} _. *)
 Global Arguments gen_token_name {Σ} _.
 Global Arguments gen_mem_name {Σ} _.
 Global Arguments gen_reg_name {Σ} _.
@@ -63,8 +56,6 @@ Definition ra_RXBuffer :=
   (prodR ra_TXBuffer
          (optionR (gmap_viewR VMID (optionO (prodO (leibnizO Word) (leibnizO VMID)))))).
 Definition ra_Accessible:=
-  (* (authR (gmapUR vmid (prodR dfracR (gmapUR pid  (csumR (agreeR unitO) (exclR unitO)))))). *)
-  (* (authR (gmapUR pid (prodR dfracR (csumR (agreeR unitO) (exclR unitO))))). *)
   (authR (gmapUR VMID (prodR dfracR (agreeR (gset_disjUR (leibnizO PID)))))).
 
 
@@ -73,14 +64,12 @@ Definition gen_VMΣ : gFunctors :=
   #[
       invΣ;
       na_invΣ;
-      (* GFunctor (agreeR natO); *)
-      GFunctor (frac_agreeR (leibnizO VMID));
+      GFunctor (frac_authR (agreeR (leibnizO VMID)));
       gen_heapΣ Addr Word;
       gen_heapΣ (reg_name * VMID) Word;
       GFunctor ra_TXBuffer;
       GFunctor ra_RXBuffer;
       GFunctor (authR (gmapUR VMID (prodR dfracR (agreeR (gset_disjUR (leibnizO PID))))));
-      (* GFunctor (authR (gset_disjUR (leibnizO pid))); *)
       GFunctor ra_Accessible;
       gen_heapΣ Word (VMID * Word * Word * (gmap VMID (gset PID)) * transaction_type);
       GFunctor (frac_agreeR (gset_disjR (leibnizO Word)));
@@ -90,9 +79,6 @@ Definition gen_VMΣ : gFunctors :=
 Global Instance subG_gen_VMPreG {Σ}:
   subG gen_VMΣ Σ -> gen_VMPreG Addr VMID Word reg_name PID transaction_type Σ.
 Proof.
-  (* hack: solve_inG does not currently unfold [subG X _] where X has more than
-     4 parameters. We have 6 (A, V, W, R, P, F). *)
-  (* set HA := gen_VMΣ. unfold gen_VMΣ in HA. *)
   solve_inG.
 Qed.
 
@@ -112,11 +98,10 @@ Section definitions.
   Qed.
 
   Definition get_token  (v:VMID) :=
-     (to_frac_agree (1/2) (v: leibnizO VMID)).
+     (frac_auth_auth (to_agree (v: leibnizO VMID))).
 
   Definition get_reg_gmap σ: gmap (reg_name * VMID) Word :=
      (list_to_map (flat_map (λ v, (map (λ p, ((p.1,v),p.2)) (map_to_list (get_vm_reg_file σ v)))) (list_of_vmids))).
-
 
   Definition get_txrx_auth_agree σ (f: mail_box -> PID) :
     ra_TXBuffer:=
@@ -125,10 +110,7 @@ Section definitions.
 
   Definition get_tx_agree σ := get_txrx_auth_agree σ (λ p, p.1).
 
-
   Definition get_rx_agree σ := get_txrx_auth_agree σ (λ p, p.2.1).
-
-
 
   Definition get_rx_gmap σ :=
     (Some (gmap_view_auth 1
@@ -138,46 +120,12 @@ Section definitions.
                                       | None => (v,None)
                                     end) (list_of_vmids))): (gmap VMID (optionO (prodO (leibnizO Word) (leibnizO VMID))) )))).
 
-
-  (* XXX:  seems like we have to keep resources being indexed by VMIDs...  *)
-
-  (* Definition get_owned_gset δ : (authR (gset_disjUR PID)) := *)
-  (*   (● (map_fold (λ (p:PID) (perm:permission) (s: gset_disjUR PID), *)
-  (*                 match perm.1 with *)
-  (*                 | Owned =>  match s with *)
-  (*                               | GSet s' => GSet (s' ∪ {[p]}) *)
-  (*                               | GSetBot => GSet ∅ *)
-  (*                             end *)
-  (*                 | Unowned => s *)
-  (*                end)  (GSet ∅) δ.2)). *)
-
-
-  (* Definition get_access_gmap δ : ra_Accessible := *)
-  (*   (●  (map_fold (λ (p:PID) (perm:permission) (s: (gmap PID (prodR dfracR (csumR (agreeR unitO) (exclR unitO))))), *)
-  (*                 match perm.2 with *)
-  (*                 | NoAccess => s *)
-  (*                 | SharedAccess => <[p:= ((DfracOwn 1), (Cinl (to_agree ())))]>s *)
-  (*                 | ExclusiveAccess => <[p:= ((DfracOwn 1),(Cinr (Excl ())))]>s *)
-  (*                end)  ∅  δ.2 )). *)
-
-  (* XXX: another attempt: *)
-
   Definition get_owned_gmap σ : (authR (gmapUR VMID (prodR dfracR (agreeR (gset_disjUR PID))))) :=
     (● (list_to_map (map (λ v, (v, ((DfracOwn 1),
         to_agree (GSet ((list_to_set (map (λ (p:(PID*permission)), p.1)
            (map_to_list (filter (λ p, (is_owned p.2) = true) (get_vm_page_table σ v)))))
                          : gset PID))))) (list_of_vmids)))).
 
-
-  (* Definition get_access_gmap σ : ra_Accessible := *)
-  (*   (● (list_to_map (map (λ v, (v, ((DfracOwn 1),(map_fold (λ (p:PID) (perm:permission) (s: (gset_disjUR PID)), *)
-  (*                 match (is_accessible perm) with *)
-  (*                 | false => s *)
-  (*                 | true => match s with *)
-  (*                                     | GSet s' => GSet (s' ∪ {[p]}) *)
-  (*                                     | GSetBot => GSet ∅ *)
-  (*                                   end *)
-  (*                end) (GSet ∅) (get_vm_page_table σ v))))) (list_of_VMIDs)))). *)
 
   Definition get_access_gmap σ : ra_Accessible :=
     (● (list_to_map (map (λ v, (v, ((DfracOwn 1),
@@ -203,8 +151,6 @@ Section definitions.
                   (p.1,(GSet trans.1.1.2))) (map_to_list (get_transactions σ).1))).
 
   Definition gen_vm_interp σ: iProp Σ :=
-      (* XXX: seems like (to_agree vm_count) is not very useful ...*)
-      (* own (gen_num_name vmG) (to_agree vm_count)∗ *)
       own (gen_token_name vmG) (get_token (get_current_vm σ)) ∗
       ghost_map_auth (gen_mem_name vmG) 1 (get_mem σ) ∗
       ghost_map_auth (gen_reg_name vmG) 1 (get_reg_gmap σ) ∗
@@ -214,19 +160,10 @@ Section definitions.
       own (gen_access_name vmG) (get_access_gmap σ) ∗
       ghost_map_auth (gen_trans_name vmG) 1 (get_trans_gmap σ) ∗
       own (gen_hpool_name vmG) (get_trans_gset σ) ∗
-      own (gen_retri_name vmG) (get_receivers_gmap σ)
-    .
+      own (gen_retri_name vmG) (get_receivers_gmap σ).
 
-
-  (* Definition num_agree_def (n:nat) : iProp Σ := *)
-  (*   own (gen_num_name vmG) (to_agree n). *)
-  (* Definition num_agree_aux : seal (@num_agree_def). Proof. by eexists. Qed. *)
-  (* Definition num_agree:= num_agree_aux.(unseal). *)
-  (* Definition num_agree_eq : @num_agree = @num_agree_def := num_agree_aux.(seal_eq). *)
-
-
-  Definition token_agree_def (v:VMID) : iProp Σ :=
-    own (gen_token_name vmG) (get_token v) .
+  Definition token_agree_def (v:VMID) (q:frac) : iProp Σ :=
+    own (gen_token_name vmG) (frac_auth_frag q (to_agree (v: leibnizO VMID))) .
   Definition token_agree_aux : seal (@token_agree_def). Proof. by eexists. Qed.
   Definition token_agree:= token_agree_aux.(unseal).
   Definition token_agree_eq : @token_agree = @token_agree_def := token_agree_aux.(seal_eq).
@@ -234,14 +171,12 @@ Section definitions.
 
   Definition mem_mapsto_def (a:Addr) (dq : dfrac) (w:Word) : iProp Σ :=
     (ghost_map_elem (gen_mem_name vmG) a dq w).
-    (* own (gen_mem_name vmG) (gmap_view_frag a dq (w : leibnizO Word)). *)
   Definition mem_mapsto_aux : seal (@mem_mapsto_def). Proof. by eexists. Qed.
   Definition mem_mapsto := mem_mapsto_aux.(unseal).
   Definition mem_mapsto_eq : @mem_mapsto = @mem_mapsto_def := mem_mapsto_aux.(seal_eq).
 
   Definition reg_mapsto_def (r:reg_name) (i:VMID) (dq : dfrac) (w:Word) : iProp Σ :=
     (ghost_map_elem (gen_reg_name vmG) (r,i) dq w).
-    (* own (gen_reg_name vmG) (gmap_view_frag (r,i) dq (w : leibnizO Word)). *)
   Definition reg_mapsto_aux : seal (@reg_mapsto_def). Proof. by eexists. Qed.
   Definition reg_mapsto := reg_mapsto_aux.(unseal).
   Definition reg_mapsto_eq : @reg_mapsto = @reg_mapsto_def := reg_mapsto_aux.(seal_eq).
@@ -273,26 +208,10 @@ Section definitions.
 
   Definition owned_mapsto_def (i:VMID) dq (s: gset_disj PID) : iProp Σ :=
     own (gen_owned_name vmG) (◯ {[i := (dq, to_agree s)]}).
-  (* Definition owned_mapsto_def (s: gset_disj PID) : iProp Σ := *)
-    (* own (gen_owned_name vmG) (◯ s). *)
   Definition owned_mapsto_aux : seal (@owned_mapsto_def). Proof. by eexists. Qed.
   Definition owned_mapsto := owned_mapsto_aux.(unseal).
   Definition owned_mapsto_eq : @owned_mapsto = @owned_mapsto_def := owned_mapsto_aux.(seal_eq).
 
-  (* Definition access_mapsto_def (i:VMID) dq (m: gmap PID access) : iProp Σ := *)
-  (*   own (gen_access_name vmG) (◯ {[i := (dq, (map_fold (λ p a acc, *)
-  (*                                                      match a with *)
-  (*                                                        | NoAccess => acc *)
-  (*                                                        | SharedAccess => <[p:=(Cinl (to_agree ()))]>acc *)
-  (*                                                        | ExclusiveAccess => <[p:=(Cinr (Excl ()))]>acc *)
-  (*                                                      end) ∅ m))]}). *)
-  (* Definition access_mapsto_def dq (m: gmap PID access) : iProp Σ := *)
-  (*   own (gen_access_name vmG) (◯ (map_fold (λ p a acc, *)
-  (*                                                      match a with *)
-  (*                                                        | NoAccess => acc *)
-  (*                                                        | SharedAccess => <[p:=(dq, (Cinl (to_agree ())))]>acc *)
-  (*                                                        | ExclusiveAccess => <[p:=(dq, (Cinr (Excl ())))]>acc *)
-  (*                                                      end) ∅ m)). *)
   Definition access_mapsto_def (i:VMID) dq (s: gset_disj PID) : iProp Σ :=
     own (gen_access_name vmG) (◯ {[i := (dq, to_agree s)]}).
   Definition access_mapsto_aux : seal (@access_mapsto_def). Proof. by eexists. Qed.
@@ -319,14 +238,10 @@ Section definitions.
 
 End definitions.
 
-(* predicate for the number of vms *)
-(* Notation "## n" := (num_agree n) *)
-(*                         (at level 50, format "## n"): bi_scope. *)
-
 (* predicate for current vm (token) *)
 
-Notation "<< n >>" := (token_agree n)
-                        (at level 50, format "<< n >>"): bi_scope.
+Notation "<< n >>{ q }" := (token_agree n q)
+                        (at level 50, format "<< n >>{ q  }"): bi_scope.
 
 (* point-to predicates for registers and memory *)
 Notation "r @@ i ->r{ q } w" := (reg_mapsto r i (DfracOwn q) w)
@@ -378,56 +293,93 @@ Section hyp_lang_rules.
   Implicit Types w: Word.
 
 
-  Lemma token_valid i1 i2 :
-   << i1 >> -∗
-      << i2 >> -∗
-      ⌜ i1 = i2 ⌝.
+  Lemma token_frag_valid i1 i2 q1 q2 :
+   << i1 >>{ q1 } -∗
+      << i2 >>{ q2 } -∗
+      ⌜ i1 = i2 ⌝ ∧ ⌜ ((q1 + q2) ≤ 1)%Qp ⌝.
   Proof.
     rewrite token_agree_eq /token_agree_def.
     iIntros "H1 H2".
     iDestruct (own_valid_2  with "H1 H2") as %Hvalid.
     rewrite /get_token in Hvalid.
-    apply frac_agree_op_valid_L in Hvalid.
-    destruct Hvalid;done.
+    rewrite <- frac_auth_frag_op in Hvalid.
+    apply frac_auth_frag_valid in Hvalid.
+    destruct Hvalid.
+    apply to_agree_op_inv_L in H0.
+    done.
    Qed.
 
-    Lemma token_update i1 i2 :
-   << i1 >> -∗
-      << i1 >> ==∗
-      << i2 >> ∗ << i2 >>.
+
+  Lemma token_frag_split i q1 q2 :
+   (q1 + q2 = 1)%Qp ->
+   << i >>{ 1%Qp } -∗
+      << i >>{ q1 } ∗ << i >>{ q2}.
+  Proof.
+    intro.
+    rewrite token_agree_eq /token_agree_def.
+    iIntros "H".
+    rewrite -own_op.
+    rewrite -frac_auth_frag_op.
+    rewrite H.
+    by rewrite agree_idemp.
+   Qed.
+
+   Lemma token_frag_merge i q1 q2 :
+   (q2 + q1 = 1)%Qp ->
+      << i >>{ q1 } -∗ << i >>{ q2} -∗
+   << i >>{ 1%Qp }.
+  Proof.
+    intro.
+    rewrite token_agree_eq /token_agree_def.
+    iIntros "H1 H2".
+    iDestruct (own_op with "[H1 H2]") as "H".
+    iFrame.
+    rewrite -frac_auth_frag_op.
+    rewrite H.
+    by rewrite agree_idemp.
+   Qed.
+
+
+   Lemma token_auth_valid i1 i2 q :
+   << i1 >>{ q } -∗
+      (own (gen_token_name vmG) (get_token i2)%I) -∗
+      ⌜ i1 = i2 ⌝.
+  Proof.
+    rewrite token_agree_eq /token_agree_def.
+    iIntros "H1 H2".
+    iDestruct (own_valid_2  with "H2 H1") as %Hvalid.
+    rewrite /get_token in Hvalid.
+    apply frac_auth_included_total in Hvalid.
+    apply to_agree_included in Hvalid.
+    destruct Hvalid.
+    done.
+   Qed.
+
+
+    Lemma token_update i1 i2 i3 :
+   << i1 >>{ 1%Qp } -∗
+      (own (gen_token_name vmG) (get_token i2))  ==∗
+      << i3 >>{ 1%Qp } ∗ (own (gen_token_name vmG) (get_token i3)).
   Proof.
     rewrite token_agree_eq /token_agree_def /get_token.
     rewrite -own_op.
     iApply own_update_2.
-    rewrite - frac_agree_op.
-    pose proof (to_frac_agree_exclusive (i1: leibnizO VMID)).
-    assert (Heq:  ( 1/2 + 1/2 =  1)%Qp ).
-    { apply (bool_decide_unpack _). by compute. }
-    rewrite Heq.
-    apply (cmra_update_exclusive ).
-    rewrite -frac_agree_op.
-    unfold to_frac_agree.
-    rewrite Heq.
-    apply pair_valid.
-    split;done.
+   apply frac_auth_update_1.
+   done.
   Qed.
 
-   Lemma gen_token_valid_neq{σ} i j:
+   Lemma gen_token_valid_neq{σ q} i j:
    i ≠ j ->
-   << i >> -∗
+   << i >>{ q } -∗
    own (gen_token_name vmG) (get_token (get_current_vm σ)) -∗
    ⌜ ¬ scheduler σ j ⌝.
   Proof.
     iIntros (Hne) "Htok Hstate".
-    rewrite token_agree_eq /token_agree_def.
-     iDestruct (own_valid_2  with "Htok Hstate") as %Hvalid.
-    rewrite /get_token in Hvalid.
-    apply frac_agree_op_valid_L in Hvalid.
-    destruct Hvalid.
+    iDestruct (token_auth_valid with "Htok Hstate") as %->.
     iPureIntro.
-    rewrite /scheduler -H0.
+    rewrite /scheduler .
     intro.
-    apply fin_to_nat_inj in H1.
+    apply fin_to_nat_inj in H.
     done.
     Qed.
 
@@ -798,69 +750,6 @@ Proof.
   - apply (H a2 w2);eauto.
     by simplify_map_eq.
  Qed.
-
-(* Program Definition p0 := (@nat_to_fin 0 page_size _). *)
-(* Program Definition p1 := (@nat_to_fin 1 page_size _). *)
-(* Program Definition p2 := (@nat_to_fin 2 page_size _). *)
-(* Program Definition p3 := (@nat_to_fin 3 page_size _). *)
-(* Program Definition p4 := (@nat_to_fin 4 page_size _). *)
-(* Program Definition p5 := (@nat_to_fin 5 page_size _). *)
-(* Program Definition p6 := (@nat_to_fin 6 page_size _). *)
-(* Program Definition p7 := (@nat_to_fin 7 page_size _). *)
-(* Solve All Obligations with *)
-(*     (intros;pose proof (page_size_at_least);assert(H': page_size_lower_bound=15);first done;lia). *)
-
-(* Program Definition new_transaction_descriptor11 p v wf wh wt wc rcvr p' := *)
-(*  ((page_offset_to_Addr p p0)->a encode_VMID v ∗ *)
-(*  (page_offset_to_Addr p p1)->a wf ∗ *)
-(*  (page_offset_to_Addr p p2)->a wh ∗ *)
-(*  (page_offset_to_Addr p p3)->a wt ∗ *)
-(*  (page_offset_to_Addr p p4)->a wc ∗ *)
-(*  (page_offset_to_Addr p p5)->a one_Word ∗ *)
-(*  (page_offset_to_Addr p p6)->a encode_VMID rcvr ∗ *)
-(*  (page_offset_to_Addr p p7)->a encode_PID p')%I. *)
-
-(* Lemma gen_mem_valid_td11: *)
-(*   ∀ (σ : state) ptx i wf wh wt j pd, *)
-(*     new_transaction_descriptor11 ptx i wf wh wt one_Word j pd -∗ *)
-(*     ghost_map_auth (gen_mem_name vmG) 1 (get_mem σ) -∗ *)
-(*     ⌜ (get_mem σ) !! (page_offset_to_Addr ptx p0) = Some (encode_VMID i) ⌝ *)
-(*     ∗ ⌜ (get_mem σ) !! (page_offset_to_Addr ptx p1) = Some wf ⌝ *)
-(*     ∗ ⌜ (get_mem σ) !! (page_offset_to_Addr ptx p2) = Some wh ⌝ *)
-(*     ∗ ⌜ (get_mem σ) !! (page_offset_to_Addr ptx p3) = Some wt ⌝ *)
-(*     ∗ ⌜ (get_mem σ) !! (page_offset_to_Addr ptx p4) = Some one_Word ⌝ *)
-(*     ∗ ⌜ (get_mem σ) !! (page_offset_to_Addr ptx p5) = Some one_Word ⌝ *)
-(*     ∗ ⌜ (get_mem σ) !! (page_offset_to_Addr ptx p6) = Some (encode_VMID j) ⌝ *)
-(*     ∗ ⌜ (get_mem σ) !! (page_offset_to_Addr ptx p7) = Some (encode_PID pd) ⌝. *)
-(* Proof. *)
-(*   iIntros (????????) "Htd Hσ". *)
-(*   rewrite /new_transaction_descriptor11 . *)
-(*   iDestruct (gen_mem_valid_Sep _ {[(page_offset_to_Addr ptx p0):= encode_VMID i; *)
-(*                                    (page_offset_to_Addr ptx p1):= wf; *)
-(*                                    (page_offset_to_Addr ptx p2):= wh; *)
-(*                                    (page_offset_to_Addr ptx p3):= wt; *)
-(*                                    (page_offset_to_Addr ptx p4):= one_Word ; *)
-(*                                    (page_offset_to_Addr ptx p5):= one_Word ; *)
-(*                                    (page_offset_to_Addr ptx p6):= encode_VMID j; *)
-(*                                    (page_offset_to_Addr ptx p7):= encode_PID pd]} with "Hσ [Htd]") as "%";eauto. *)
-(*   rewrite !big_sepM_insert ?big_sepM_empty;eauto;first *)
-(*   (iDestruct "Htd" as "(?&?&?&?&?&?&?&?)"; *)
-(*   iFrame); *)
-(*   repeat rewrite lookup_insert_ne;first done;repeat (apply  page_offset_to_Addr_neq;eauto);done. *)
-(*   iPureIntro. *)
-(*   remember {[(page_offset_to_Addr ptx p0):=encode_VMID i; *)
-(*                                    (page_offset_to_Addr ptx p1):=wf; *)
-(*                                    (page_offset_to_Addr ptx p2):= wh; *)
-(*                                    (page_offset_to_Addr ptx p3):= wt; *)
-(*                                    (page_offset_to_Addr ptx p4):= one_Word ; *)
-(*                                    (page_offset_to_Addr ptx p5):= one_Word ; *)
-(*                                    (page_offset_to_Addr ptx p6):= encode_VMID j; *)
-(*                                    (page_offset_to_Addr ptx p7):= encode_PID pd]} as m. *)
-(*   repeat (try split); *)
-(*   apply (map_Forall_lookup_1 (λ (k : Addr) (x : Word), get_mem σ !! k = Some x) m );eauto; *)
-(*   simplify_eq /=; repeat try (simplify_map_eq;try done;try (rewrite lookup_insert_ne; simplify_map_eq;try done)); *)
-(*   apply page_offset_to_Addr_neq;eauto;done. *)
-(* Qed. *)
 
 
 Lemma gen_mem_update1:
@@ -1445,7 +1334,7 @@ Qed.
     done.
   Qed.
 
-  Global Instance token_timeless i : Timeless (<<i>>).
+  Global Instance token_timeless i q : Timeless (<<i>>{ q }).
   Proof. rewrite token_agree_eq /token_agree_def. apply _. Qed.
 
   Global Instance mem_mapsto_timeless a q w : Timeless ((a ->a{q} w)).
