theories/examples/run_yield_1.v
@@ -1,6 +1,6 @@
 From machine_program_logic.program_logic Require Import machine weakestpre.
 From HypVeri Require Import reg_addr RAs rule_misc lifting.
-From HypVeri.rules Require Import rules_base mov ldr str halt run yield.
+From HypVeri.rules Require Import rules_base mov halt run yield.
 From iris.proofmode Require Import tactics.
 From iris.base_logic.lib Require Import invariants na_invariants.
 From iris.algebra Require Import excl.
@@ -50,18 +50,23 @@ Section RunYield1.
 
   Definition invN := nroot .@ "tok".
 
-  Definition inv γ1 γ2 γ3 (z i:VMID) :=
-    ((∃ w0 w1, <<z>>  ∗ tokI γ1 ∗ tokI γ3 ∗ R0 @@ z ->r w0 ∗ R1 @@ z ->r w1) ∨
-     (<<z>> ∗ tokI γ2 ∗ R0 @@ z ->r yield_I ∗ R1 @@ z ->r (encode_vmid i)) ∨
-     (<<i>> ∗ tokI γ1 ∗ tokI γ2 ∗ R0 @@ z ->r run_I ∗ R1 @@ z ->r (encode_vmid i)))%I.
+  Definition na_inv γ1 γ2 γ3 (z i:VMID) :=
+    ((∃ w0 w1, <<z>>{ (1/2)%Qp }  ∗ tokI γ1 ∗ tokI γ3 ∗ R0 @@ z ->r w0 ∗ R1 @@ z ->r w1) ∨
+     (<<z>>{ (1/2)%Qp } ∗ tokI γ2 ∗ R0 @@ z ->r yield_I ∗ R1 @@ z ->r (encode_vmid i)) ∨
+     (<<i>>{ (1/2)%Qp } ∗ tokI γ1 ∗ tokI γ2 ∗ R0 @@ z ->r run_I ∗ R1 @@ z ->r (encode_vmid i)))%I.
 
-  Lemma mach_zero {γ1 γ2 γ3 z i q1 prog1page} :
+  Definition inv' :=
+    ( (∃ i, <<i>>{ (1/2)%Qp } )∨ nainv_closed ⊤ )%I.
+
+  Lemma mach_zero {γ1 γ2 γ3 z i q1 prog1page ι ι1} :
+      ι ## ι1 ->
       fin_to_nat z = 0 ->
       z ≠ i ->
       seq_in_page (of_pid prog1page) (length (program1 i)) prog1page ->
+      <<z>>{ 1%Qp } ∗
       program (program1 i) (of_pid prog1page) ∗
-      nainv invN (inv γ1 γ2 γ3 z i) ∗ tokI γ2 ∗
-      nainv_closed ⊤ ∗
+      inv ι (inv') ∗
+      nainv ι1 (na_inv γ1 γ2 γ3 z i) ∗ tokI γ2 ∗
       A@z :={q1} prog1page
       ∗ PC @@ z ->r (of_pid prog1page)
       ⊢ (WP ExecI @ z
@@ -71,14 +76,30 @@ Section RunYield1.
             ∗ A@z :={q1} prog1page
             ∗ PC @@ z ->r ((of_pid prog1page) ^+ (length (program1 i)))%f)}}%I).
   Proof.
-    iIntros (zP neH HIn) "((p_1 & p_2 & p_3 & p_4 & _) & #Hinv  & Hgtok2 & Hown & Hacc & PCz )".
+    iIntros (Hdisj zP neH HIn) "(Htok & (p_1 & p_2 & p_3 & p_4 & _) & #Hinv & #Hnainv & Hgtok2 & Hacc & PCz )".
     apply seq_in_page_forall in HIn.
-    (* mov_word_I R0 run_I *)
     rewrite wp_sswp.
-    iApply (sswp_fupd_around z ⊤ ⊤ ⊤).
-    iMod (na_inv_acc with "Hinv Hown") as "(>[HInv | [[Htok [Hgtok2' ?]] | (Htok & Hgtok1' & Hgtok2' & ?)]] & Hown & HClose)";auto.
+    (* iApply (sswp_fupd_around z ⊤ (⊤ ∖ ↑ι) ⊤). *)
+    iApply (sswp_fupd_around z ⊤ ⊤ _).
+    iInv ι as ">Inv" "HClose".
+    iDestruct "Inv" as "[Htok' | Hown ]".
+    1: {
+    iDestruct "Htok'" as (j) "Htok'".
+    iExFalso.
+    iDestruct (token_frag_valid with "Htok Htok'") as %[_ Hvalid].
+    contradiction.
+    }
+    iDestruct ((token_frag_split z (1/2)%Qp (1/2)%Qp) with "Htok") as "[Htok Htok']";try done.
+    compute_done.
+    iDestruct ("HClose" with "[Htok']") as "HIClose".
+    iNext;iLeft;iExists z;iFrame.
+    iMod "HIClose" as %_.
     iModIntro.
-    iDestruct "HInv" as (w0 w1) "( Htok & Hgtok1' & Hgtok3' & R0z & R1z )".
+    (* mov_word_I R0 run_I *)
+    iApply (sswp_fupd_around z ⊤ ⊤ _).
+    iMod (na_inv_acc with "Hnainv Hown") as "(>[HInv | [[Htok'' [Hgtok2' ?]] | (Htok'' & Hgtok1' & Hgtok2' & ?)]] & Hown & HClose)";auto.
+    (* set_solver. *)
+    iDestruct "HInv" as (w0 w1) "( Htok' & Hgtok1' & Hgtok3' & R0z & R1z )".
     2: {
       iExFalso.
       iApply (tokI_excl with "Hgtok2 Hgtok2'").
@@ -93,8 +114,10 @@ Section RunYield1.
     by rewrite decode_encode_instruction.
     by inversion HIn.
     iApply "J".
+    iModIntro.
     iNext.
     iIntros "(Htok & PCz & p_1 & Hacc & R0z)".
+    iModIntro.
     iModIntro.
     (* mov_word_I R1 (encode_vmid i) *)
     rewrite wp_sswp.
@@ -111,8 +134,8 @@ Section RunYield1.
     rewrite wp_sswp.
     iDestruct
       ((run (((of_pid prog1page) ^+ 1) ^+ 1)%f)
-         with "[Htok PCz p_3 Hacc R0z R1z]") as "J"; eauto.
-    5: { iFrame. }
+         with "[Htok Htok' PCz p_3 Hacc R0z R1z]") as "J"; eauto.
+    5: { iFrame. iNext. iApply ((token_frag_merge z (1/2)%Qp (1/2)%Qp) with "Htok Htok'"). compute_done. }
     by rewrite decode_encode_instruction.
     by inversion HIn;inversion H4; inversion H8.
     by rewrite decode_encode_hvc_func.
@@ -120,6 +143,7 @@ Section RunYield1.
     iApply "J".
     iNext.
     iIntros "(Htok & PCz & p_3 & Hacc & R0z & R1z)".
+    iDestruct ((token_frag_split i (1/2)%Qp (1/2)%Qp) with "Htok") as "[Htok Htok']". compute_done.
     iDestruct ("HClose" with "[Htok Hgtok1' Hgtok2 R0z R1z Hown]") as "Hown".
     iFrame.
     iNext.
@@ -128,9 +152,9 @@ Section RunYield1.
     iFrame.
     (* halt_I *)
     rewrite wp_sswp.
-    iApply (sswp_fupd_around z ⊤ ⊤ ⊤).
+    iApply (sswp_fupd_around z  ⊤ ⊤ _).
     iMod "Hown".
-    iMod (na_inv_acc with "Hinv Hown") as "(>[HInv | [ (Htok & Hrest) | [Htok [Hgtok2 Hrest]]]] & Hown & HClose)";auto.
+    iMod (na_inv_acc with "Hnainv Hown") as "(>[HInv | [ (Htok & Hrest) | [Htok [Hgtok2 Hrest]]]] & Hown & HClose)";auto.
     iModIntro.
     1: {
       iDestruct "HInv" as (? ?) "(_ & Hgtok1' & Hgtok3 & _ )".
@@ -155,6 +179,10 @@ Section RunYield1.
     iExFalso.
     done.
     }
+    (* XXX: we cannot continue since we have
+       "Htok'" : <<i>>{1 / 2 }
+       "Htok" : <<z>>{1 / 2 }
+     *)
     iModIntro.
     iDestruct
       ((halt ((((of_pid prog1page) ^+ 1) ^+ 1) ^+1 )%f)
@@ -314,8 +342,6 @@ Section RunYield1.
       iApply (tokI_excl with "Hgtok1 Hgtok1'").
     }
 Qed.
-
-
 
   Lemma spec1 {γ1 γ2 γ3 z i q1 q2 prog1page prog2page r0_} :
       fin_to_nat z = 0 ->
